src/Std/Do/WP.lean
@@ -9,5 +9,6 @@ prelude
 public import Std.Do.WP.Basic
 public import Std.Do.WP.Monad
 public import Std.Do.WP.SimpLemmas
+public import Std.Do.WP.Adequacy
 
 set_option linter.missingDocs true
